Work on refining click marked graph into a brick for the purposes of composition

ClickRefinement.v
@@ -15,185 +15,70 @@ Import EnsembleNotation.
 Open Scope ensemble_scope.
 Require Import Coq.Program.Equality.
 
-Section MG_to_SS.
-
-  Print marked_graph.
-  Variable name : Set.
-  Context `{name_dec : eq_dec name}.
-
-  Variable transition : Set.
-  Context `{transition_dec : eq_dec transition}.
-  Variable MG : marked_graph transition.
-
-  Variable transition_name : transition -> name.
-  Variable place_name : forall t1 t2, place MG t1 t2 -> name.
-
-  Definition places_set : Ensemble name :=
-    fun x => exists t1 t2 (p : place MG t1 t2), x = place_name _ _ p.
-  Definition state_to_marking (σ : state name) : marking MG :=
-    fun t1 t2 p => val_to_nat (σ (place_name _ _ p)).
-
-  Hypothesis name_is_place_dec : forall x,
-                           {t1 : transition & {t2 : transition
-                                            & {p : place MG t1 t2 & x = place_name _ _ p}}}
-                         + {forall t1 t2 (p : place MG t1 t2), x <> place_name _ _ p}.
-
-  Definition fire_in_state (t : transition) (σ : state name) : state name :=
-    fun x =>
-    match name_is_place_dec x with
-    (* if x is not a place, do nothign *)
-    | inright _ => σ x
-    | inleft (existT _ tin (existT _ tout (existT _ p x_is_p))) =>
-      (* corner case: do nothing *)
-      if tin =? tout then σ x
-      (* if x is a place leading into t, increment the value *)
-      else if t =? tout then dec_value (σ x)
-      (* if x is a place leading out of t, decrement the value *)
-      else if t =? tin then inc_value (σ x)
-      (* otherwise do nothing *)
-      else σ x
-    end.
-
-  Variable transition_update_value : transition -> value -> value.
-  (* Condition: input_transition, output_transition should partition the set of all transitions *)
-  Variable input_transition : Ensemble transition.
-  Variable output_transition : Ensemble transition.
-
-  Inductive MG_SS_step
-    : state name -> option (event name value) -> option (state name) -> Prop :=
-
-  | transition_enabled σ σ' x v (t : transition) :
-    x = transition_name t ->
-    is_enabled MG t (state_to_marking σ) ->
-    v = transition_update_value t (σ x) ->
-    σ' = update (fire_in_state t σ) x v ->
-    MG_SS_step σ (Some (Event x v)) (Some σ')
-
-  | input_not_enabled σ x v t :
-    x = transition_name t ->
-    t ∈ input_transition ->
-    ~ is_enabled MG t (state_to_marking σ) ->
-   MG_SS_step σ (Some (Event x v)) None
-  .
-
-  Definition MG_SS : StateSpace name :=
-  {| space_input := fmap transition_name input_transition
-   ; space_output := fmap transition_name output_transition
-   ; space_internal := places_set
-   ; space_step := MG_SS_step
-   |}.
-
-End MG_to_SS.
-
 Section ClickRefinement.
 
-Variable name : Set.
-Context `{name_dec : eq_dec name}.
-Variable even odd : Set.
-Context `{scheme : naming_scheme name even odd}.
+  Variable even odd : Set.
+  Variable name : Set.
+  Context `{name_dec : eq_dec name}.
+  Context `{scheme : naming_scheme name even odd}
+          `{x_scheme : stage_naming_scheme name even odd}.
 
-Variable l : latch even odd.
-
-(** Define a state space [latch_stage_refinement such that every trace accepted
-by [latch_stage l] is also accepted by [latch_stage_refinement l] *)
-
-Require Import ClickMG. 
-Class extended_naming_scheme :=
-    {place_name : forall {t1 t2 : token_transition}, stage_place t1 t2 -> name}.
-Context `{extended_naming_scheme}.
-Print stage_place.
-Definition name_is_place_dec : forall x,
-                          {t1 : token_transition &
-                           {t2 : token_transition & {p : stage_place t1 t2 & x = place_name p}}}
-                        + {forall t1 t2 (p : stage_place t1 t2), x <> place_name p}.
-Proof.
-  intros x. Print stage_place.
-
-  Ltac compare_place_name x p :=
-    compare x (place_name p);
-      [ left; do 3 eexists; reflexivity | ].
-  compare_place_name x left_ack_left_req.
-  compare_place_name x clk_fall_left_req.
-  compare_place_name x right_req_left_req.
-  compare_place_name x clk_rise_left_ack.
-  compare_place_name x clk_rise_right_req.
-  compare_place_name x right_req_right_ack.
-  compare_place_name x clk_fall_right_ack.
-  compare_place_name x left_ack_right_ack.
-  compare_place_name x clock_fall.
-  compare_place_name x left_req_clk_rise.
-  compare_place_name x right_ack_clk_rise.
-  right. intros t1 t2 p; destruct p; auto.
-Defined.
+  Definition input_environment (h : handshake name) : StateSpace name :=
+    NOT (ack h) (req h).
+  Definition output_environment (h : handshake name) : StateSpace name :=
+    forward (req h) (ack h).
+  Definition brick_stage (hin hout : handshake name) : StateSpace name :=
+      input_environment hin
+    ∥ output_environment hout
+    ∥ forward (req hin) (req hout)
+    ∥ forward (ack hout) (ack hin).
+  Lemma brick_stage_input : forall hin hout, 
+    all_disjoint [req hin; req hout; ack hin; ack hout] ->
+    space_input (brick_stage hin hout) == ∅.
+  Proof.
+    intros.
+    constructor.
+    * intros x Hx; simpl in *; decompose_set_structure; solve_set.
+    * intros x Hx. inversion Hx.
+  Qed.
+  Lemma brick_stage_output : forall hin hout, 
+    all_disjoint [req hin; req hout; ack hin; ack hout] ->
+    space_output (brick_stage hin hout) == from_list [req hin; req hout; ack hin; ack hout].
+  Proof.
+    intros.
+    constructor;
+      intros x Hx; simpl in *; decompose_set_structure; solve_set.
+  Qed.
 
 
-Definition places_set : Ensemble name :=
-  fun x => exists t1 t2 (p : stage_place t1 t2), x = place_name p.
+  Variable l : latch even odd. Print naming_scheme. About NOT.
+  Let out_flag := latch_to_token_flag l.
+  (* in_flag is opposite of out_flag here *)
+  Let in_flag := match l with
+                 | Odd _ => Token
+                 | Even _ => NonToken
+                 end.
 
-
-
-Definition state_to_marking (σ : state name) : marking stage_MG :=
-  fun t1 t2 p => val_to_nat (σ (place_name p)).
-Print naming_scheme. Print token_transition.
-Print stage_MG. Print stage_place. Print value. Print enumerate.
-Arguments enumerate A {enumerable}.
-Print sig.
-  
-
-(** A transition should only fire if the caller has independently checked that it
-  is enabled. *) Print sigT. Print sumor.
-Search eq_dec token_transition.
-Existing Instance token_transition_eq_dec.
-Program Definition fire_in_state (t : token_transition) (σ : state name) : state name :=
-  fun x =>
-    match name_is_place_dec x with
-    (* if x is not a place, do nothign *)
-    | inright _ => σ x
-    | inleft (existT _ tin (existT _ tout (existT _ p x_is_p))) =>
-      (* corner case: do nothing *)
-      if tin =? tout then σ x
-      (* if x is a place leading into t, increment the value *)
-      else if t =? tout then dec_value (σ x)
-      (* if x is a place leading out of t, decrement the value *)
-      else if t =? tin then inc_value (σ x)
-      (* otherwise do nothing *)
-      else σ x
-    end.
-
-Print transition_name.
-Arguments transition_name {name even odd H0}.
-
-
-Inductive latch_step_refinement
-  : state name -> option (event name value) -> option (state name) -> Prop :=
-
-| transition_enabled σ σ' x v (t : token_transition) :
-  x = transition_name l t ->
-  is_enabled stage_MG t (state_to_marking σ) ->
-  v = transition_update_value t (σ x) ->
-  σ' = update (fire_in_state t σ) x v ->
-  latch_step_refinement σ (Some (Event x v)) (Some σ')
-
-| input_not_enabled σ x v t :
-  x ∈ space_input (latch_stage l) ->
-  x = transition_name l t ->
-  ~ is_enabled stage_MG t (state_to_marking σ) ->
-  latch_step_refinement σ (Some (Event x v)) None
-.
-
-
-
-(** the internal wires are all the wire names corresponding to places in the
-marked graph *)
-
-
-
-Definition latch_state_refinement : StateSpace name :=
-  {| space_input := space_input (latch_stage l)
-   ; space_output := space_output (latch_stage l)
-   ; space_internal := places_set 
-   ; space_step := latch_step_refinement
-   |}.
+About traces_of.
+Arguments traces_of {name}.
+About stage_MG_SS.
+Arguments stage_MG_SS {name} {name_dec} {even odd} l f {scheme x_scheme} : rename.
+About init_stage_MG_state.
+Arguments init_stage_MG_state {name name_dec even odd scheme x_scheme} : rename.
+  Lemma stage_is_brick :
+      traces_of (hide (latch_clk l) (stage_MG_SS l in_flag)) (init_stage_MG_state l)
+    ⊆ traces_of (brick_stage (latch_input l) (latch_output l)) (σR l).
+  Proof.
+    Search traces_of.
+    apply relate_trace_step_subset.
+    * admit (* true *).
+    * unfold relate_trace_step_lemma.
+      intros σ1 σ1' σ2 e t Hstep Hrelate.
+      inversion Hstep; subst.
+      inversion H1; subst.
+      (* seems easier to reason about if brick_stage is a marked graph *)
+      admit.
+  Admitted.
 
 
 End ClickRefinement.
